@prefix rdfg: <http://www.w3.org/2004/03/trix/rdfg-1/> .
@prefix rdfs: <http://www.w3.org/2000/01/rdf-schema#> .
@prefix rdf: <http://www.w3.org/1999/02/22-rdf-syntax-ns#> .
@prefix xsd: <http://www.w3.org/2001/XMLSchema#> .
@prefix owl: <http://www.w3.org/2002/07/owl#> .

@prefix cc: <http://creativecommons.org/ns#> .

@prefix doaj: <https://doaj.org/> .

@prefix dc: <http://purl.org/dc/elements/1.1/> .

@prefix dcterms: <http://purl.org/dc/terms/> .

@prefix fabio: <http://purl.org/spar/fabio/> .

@prefix ppo: <https://purl.org/cwts/ppo/> .

@prefix pro: <https://purl.org/spar/pro/> .

@prefix loc: <http://id.loc.gov/ontologies/bibframe/> .

@prefix openalex: <https://openalex.org/> .

@prefix prism: <http://prismstandard.org/namespaces/basic/2.0/> .

@prefix romeo: <https://v2.sherpa.ac.uk/id/> .

@prefix schema: <https://schema.org/> .

@prefix wd: <http://www.wikidata.org/entity/> .

@prefix xsd: <http://www.w3.org/2001/XMLSchema#> .

ppo:Platform a rdfs:Class ;
    rdfs:label "Platform"@en ;
    rdfs:comment "A platform that plays some role in the publishing process (e.g. publication, hosting, reviewing, etc.)."@en .

ppo:PlatformType a rdfs:Class ;
    rdfs:label "Platform Type"@en ;
    rdfs:comment "The role that a platform can fulfill during the publication process."@en .

ppo:Policy a rdfs:Class ;
    rdfs:label "Policy"@en ;
    rdfs:comment "A collection of rules and allowances that the platform maintains."@en .

ppo:PublicationPolicy rdfs:subClassOf ppo:Policy ;
    rdfs:label "Publication Policy"@en ;
    rdfs:comment "Rules and allowances that a platform maintains during the publication of a scholarly article."@en .

ppo:EvaluationPolicy rdfs:subClassOf ppo:Policy ;
    rdfs:label "Evaluation Policy"@en ;
    rdfs:comment "Rules and allowances that a platform maintains during the evaluation of a scholarly article."@en .

ppo:PublicationElsewherePolicy rdfs:subClassOf ppo:Policy ;
    rdfs:label "Publication Elsewhere Policy"@en ;
    rdfs:comment "Rules and allowances that a platform maintains with regard to other platforms."@en .

ppo:hasPlatformType a rdf:Property ;
    rdfs:domain ppo:Platform ;
    rdfs:range ppo:PlatformType ;
    rdfs:label "has Platform Type"@en ;
    rdfs:comment "The property relating a Platform to a specific platform type."@en .

ppo:hasPolicy a rdf:Property ;
    rdfs:domain ppo:Platform, ppo:PlatformType ;
    rdfs:range ppo:Policy ;
    rdfs:label "has Policy"@en ;
    rdfs:comment "The property relating a Platform to a specific Policy."@en .

ppo:documentVersion a rdf:Class ;
    rdfs:label "Document version"@en ;
    rdfs:comment "The version of a publishable document."@en .

ppo:publishedVersion a ppo:documentVersion ;
    rdfs:label "Published version"@en ;
    rdfs:comment "The published version of a publishable document."@en .

ppo:acceptedVersion a ppo:documentVersion ;
    rdfs:label "Accepted version"@en ;
    rdfs:comment "The accepted version of a publishable document."@en .

ppo:submittedVersion a ppo:documentVersion ;
    rdfs:label "Submitted version"@en ;
    rdfs:comment "The submitted version of a publishable document."@en .

ppo:anonymousTo a rdf:Property ;
    rdfs:domain pro:PublishingRole ;
    rdfs:range pro:PublishingRole ;
    rdfs:label "Anonymous To"@en ;
    rdfs:comment "The relation that signifies that the subject is not aware of the identity of the object."@en .

ppo:interactsWith a owl:SymmetricProperty ;
    rdfs:domain pro:PublishingRole ;
    rdfs:range pro:PublishingRole ;
    rdfs:label "The relation that signifies that the subject can interact with the object during the review process."@en ;
    rdfs:comment ""@en .

ppo:possibleDecision a rdf:Property ;
    rdfs:domain ppo:EvaluationPolicy ;
    rdfs:range xsd:String ;
    rdfs:label "possible Decision"@en ;
    rdfs:comment "Relation that describes the possible decision that can be made during the evaluation of a work by the platform."@en .

ppo:involves a rdf:Property ;
    rdfs:domain ppo:Policy ;
    rdfs:range pro:PublishingRole ;
    rdfs:label "involves"@en ;
    rdfs:comment "Relation that describes that the object is involved during the process for a specific policy."@en .

ppo:hasInitiator rdfs:subPropertyOf ppo:involves ;
    rdfs:domain ppo:EvaluationPolicy ;
    rdfs:range pro:PublishingRole ;
    rdfs:label "has Initiator"@en ;
    rdfs:comment "Relation that describes the object as the initiator for a specific evaluation policy."@en .

ppo:covers a rdf:Property ;
    rdfs:domain ppo:EvaluationPolicy ;
    rdfs:range ppo:DocumentType ;
    rdfs:label "covers"@en ;
    rdfs:comment "Relation that signifies that a policy includes restrictions or allowances on a particular type of document related to the work or policy."@en .

ppo:PublicAccessability a rdfs:Class ;
    rdfs:label "Public Accessibility"@en ;
    rdfs:comment "Status that a work can have regarding its public availability."@en .

ppo:Accessible a owl:NamedIndividual ;
    rdfs:label "Accessible"@en ;
    rdfs:comment "The work is made publicly available."@en .

ppo:NotAccessible a owl:NamedIndividual ;
    rdfs:label "Not Accessible"@en ;
    rdfs:comment "The work is not made publicly available."@en .

ppo:OptIn a rdfs:Class ;
    rdfs:label "Opt-In"@en ;
    rdfs:comment "The work is made publicly available with the permission of all persons holding a publishing role that has an ppo:optInBy relation with this individual."@en .

ppo:publiclyAccessible a rdf:Property ;
    rdfs:domain fabio:Work ;
    rdfs:range ppo:PublicAccessability ;
    rdfs:label "publicly Accessible"@en ;
    rdfs:comment "Relation that signifies the public availability of the Document."@en .

ppo:identityPubliclyAccessible a rdf:Property ;
    rdfs:domain pro:PublishingRole ;
    rdfs:range ppo:PublicAccessability ;
    rdfs:subPropertyOf ppo:publiclyAccessible ;
    rdfs:label "identity Publicly Accessible"@en ;
    rdfs:comment "Relation that signifies the public availability of the publishing role."@en .

ppo:optInBy a rdf:Property ;
    rdfs:domain ppo:OptIn ;
    rdfs:range pro:PublishingRole ;
    rdfs:label "opt-In By"@en ;
    rdfs:comment "Relation that signifies the permission of persons holding a publishing role for a specific thing to be made publicly accessible."@en .

ppo:hasOpenalexId a rdf:Property ;
    rdfs:subPropertyOf dcterms:identifier ;
    rdfs:domain ppo:Platform ;
    rdfs:range xsd:anyURI ;
    rdfs:label ""@en ;
    rdfs:comment ""@en .

ppo:hasFatcatId a rdf:Property ;
    rdfs:subPropertyOf dcterms:identifier ;
    rdfs:domain ppo:Platform ;
    rdfs:range xsd:anyURI ;
    rdfs:label ""@en ;
    rdfs:comment ""@en .

ppo:hasWikidataId a rdf:Property ;
    rdfs:subPropertyOf dcterms:identifier ;
    rdfs:domain ppo:Platform ;
    rdfs:range xsd:anyURI ;
    rdfs:label ""@en ;
    rdfs:comment ""@en .

dcterms:license a rdf:Property ;
    rdfs:domain ppo:Assertion ;
    rdfs:range xsd:IRI ;
    rdfs:isDefinedBy <http://purl.org/dc/elements/1.1/license> .

cc:license rdfs:subPropertyOf dcterms:license .

dcterms:created a rdf:Property ;
    rdfs:domain ppo:Assertion ;
    rdfs:range xsd:DateTime ;
    rdfs:isDefinedBy <http://purl.org/dc/elements/1.1/created> .

dcterms:creator a rdf:Property ;
    rdfs:domain ppo:Assertion ;
    rdfs:range dcterms:Agent ;
    rdfs:isDefinedBy <http://purl.org/dc/elements/1.1/creator> .

dcterms:publisher a rdf:Property ;
    rdfs:domain ppo:Platform ;
    rdfs:range dcterms:Agent ;
    rdfs:isDefinedBy <http://purl.org/dc/elements/1.1/publisher> .

dcterms:identifier a rdf:Property ;
    rdfs:domain ppo:Platform ;
    rdfs:range xsd:Literal ;
    rdfs:isDefinedBy <http://purl.org/dc/elements/1.1/identifier> .

fabio:hasIssnL a rdf:Property ;
    rdfs:subPropertyOf dcterms:identifier ;
    rdfs:domain ppo:Platform ;
    rdfs:range xsd:String ;
    rdfs:label ""@en ;
    rdfs:comment ""@en .

prism:issn a rdf:Property ;
    rdfs:subPropertyOf dcterms:identifier ;
    rdfs:domain ppo:Platform ;
    rdfs:range xsd:String ;
    rdfs:label ""@en ;
    rdfs:comment ""@en .

prism:eIssn a rdf:Property ;
    rdfs:subPropertyOf dcterms:identifier ;
    rdfs:domain ppo:Platform ;
    rdfs:range xsd:String ;
    rdfs:label ""@en ;
    rdfs:comment ""@en .

prism:doi a rdf:Property ;
    rdfs:subPropertyOf dcterms:identifier ;
    rdfs:domain ppo:Platform ;
    rdfs:range xsd:String ;
    rdfs:label ""@en ;
    rdfs:comment ""@en .

romeo:id a rdf:Property ;
    rdfs:subPropertyOf dcterms:identifier ;
    rdfs:domain ppo:Platform ;
    rdfs:range xsd:anyURI ;
    rdfs:label ""@en ;
    rdfs:comment ""@en .

wd:id a rdf:Property ;
    rdfs:subPropertyOf dcterms:identifier ;
    rdfs:domain ppo:Platform ;
    rdfs:range xsd:String ;
    rdfs:label ""@en ;
    rdfs:comment ""@en .

schema:name a rdf:Property ;
    rdfs:domain ppo:Platform ;
    rdfs:range xsd:String ;
    rdfs:isDefinedBy <http://schema.org/name> .

pro:PublishingRole a rdfs:Class ;
    rdfs:isDefinedBy <https://purl.org/spar/pro/PublishingRole> .

pro:author a pro:PublishingRole ;
    rdfs:isDefinedBy <https://purl.org/spar/pro/author> .

pro:peer-reviewer a pro:PublishingRole ;
    rdfs:isDefinedBy <https://purl.org/spar/pro/peer-reviewer> .

pro:editor a pro:PublishingRole ;
    rdfs:isDefinedBy <https://purl.org/spar/pro/editor> .

pro:publisher a pro:PublishingRole ;
    rdfs:isDefinedBy <https://purl.org/spar/pro/publisher> .

fabio:Work a rdfs:Class ;
    rdfs:isDefinedBy <http://purl.org/spar/fabio/Work> .

ppo:ReviewReport a fabio:Work, owl:NamedIndividual ;
    rdfs:isDefinedBy <https://osf.io/7j6ck> ;
    rdfs:label "Review Report"@en .

ppo:ReviewSummary a fabio:Work, owl:NamedIndividual ;
    rdfs:isDefinedBy <https://osf.io/7j6ck> ;
    rdfs:label "Review Summary"@en .

ppo:AuthorEditorCommunication a fabio:Work, owl:NamedIndividual ;
    rdfs:isDefinedBy <https://osf.io/7j6ck> ;
    rdfs:label "Author-Editor Communication"@en .

ppo:SubmittedManuscript a fabio:Work, owl:NamedIndividual ;
    rdfs:isDefinedBy <https://osf.io/7j6ck> ;
    rdfs:label "Submitted Manuscript"@en .
